Convert to partial memory representation.
As per our meeting on 2012-02-03, we converted the memory representation
in IL.v from total (W -> B) to partial (W -> option B).  We modified
the ReadWord primitive to be partial, and fixed up all of the main Bedrock
theorems that broke in the process.  Overall, this translation was
fairly pleasant.

This patch is incomplete, it does not:

    - Remove the now irrelevant inBounds checking
    - Add new predicates for properly asserting that a memory is
      appropriately total.  We may just want to do exists and ===>
    - Figure out why the 'ho' tactic stopped working

src/SepIL.v
@@ -1,5 +1,5 @@
 Require Import Eqdep_dec List.
-Require Import Word PropX PropXTac IL DepList Heaps SepTheoryX.
+Require Import Word Memory PropX PropXTac IL Bedrock.DepList Heaps SepTheoryX.
 
 Set Implicit Arguments.
 
@@ -13,13 +13,13 @@ Fixpoint allWordsUpto (width init : nat) : list (word width) :=
 Definition allWords_def (width : nat) :=
   allWordsUpto width (pow2 width).
 
-Fixpoint memoryInUpto (width init : nat) (memHigh : word width) (m : word width -> B)
+Fixpoint memoryInUpto (width init : nat) (memHigh : word width) (m : word width -> option B)
   : hlist (fun _ => option B) (allWordsUpto width init) :=
   match init with
     | O => HNil
     | S init' =>
       let w := natToWord width init' in
-        let v := if wlt_dec w memHigh then if wlt_dec (w ^+ $3) memHigh then Some (m w) else None else None in
+        let v := if wlt_dec w memHigh then if wlt_dec (w ^+ $3) memHigh then m w else None else None in
           HCons v (memoryInUpto (width := width) init' memHigh m)
   end.
 
@@ -37,7 +37,7 @@ Module Type ALL_WORDS.
 
   Axiom allWords_eq : allWords = allWords_def.
 
-  Parameter memoryIn : forall width, word width -> (word width -> B) -> hlist (fun _ => option B) (allWords width).
+  Parameter memoryIn : forall width, word width -> (word width -> option B) -> hlist (fun _ : word width => option B) (allWords width).
 
   Axiom memoryIn_eq : forall width,
     memoryIn (width := width)
@@ -123,10 +123,10 @@ Module BedrockHeap.
 
   Definition mem := mem.
 
-  Definition mem_get (m : mem) (a : addr) := Some (m a).
+  Definition mem_get (m : mem) (a : addr) := m a.
 
   Definition mem_set (m : mem) (p : addr) (v : B) := 
-    fun p' => if weq p p' then v else m p'.
+    fun p' => if weq p p' then Some v else m p'.
 
   Theorem mem_get_set_eq : forall m p v', 
     mem_get (mem_set m p v') p = Some v'.
@@ -170,6 +170,7 @@ Import ST.HT.
 Export ST.HT.
 
 (** * Define some convenient connectives, etc. for specs *)
+
 Definition memoryIn : W -> mem -> smem := memoryIn (width := 32).
 
 Definition hpropB := hprop W (settings * state).
@@ -451,7 +452,7 @@ Qed.
 
 Lemma smem_get'_read : forall a v (memHigh : W) m init,
   smem_get' _ a (memoryInUpto init memHigh m) = Some v
-  -> m a = v.
+  -> m a = Some v.
   induction init.
   simpl; congruence.
   unfold allWordsUpto.
@@ -464,13 +465,12 @@ Lemma smem_get'_read : forall a v (memHigh : W) m init,
   unfold hlist_hd in H.
   congruence.
   discriminate.
-  discriminate.
-  auto.
+  destruct (m a); auto.
 Qed.
 
 Lemma smem_get_read : forall stn a v m,
   smem_get a (memoryIn (MemHigh stn) m) = Some v
-  -> m a = v.
+  -> m a = Some v.
   unfold memoryIn; rewrite AllWords.memoryIn_eq; intros ? ? ? ?.
   unfold smem_get, BedrockHeap.all_addr.
   match goal with
@@ -485,7 +485,7 @@ Qed.
 Theorem findPtsto8_read : forall specs p st,
   interp specs (sepFormula p st)
   -> forall a v, findPtsto8 p a v
-    -> Mem (snd st) a = v.
+    -> Mem (snd st) a = Some v.
   rewrite sepFormula_eq; intros.
   apply H0 in H.
   eapply smem_get_read; eauto.
@@ -548,14 +548,14 @@ Qed.
 Theorem findPtsto32_read : forall specs p stn st,
   interp specs (sepFormula p (stn, st))
   -> forall a v, findPtsto32 stn p a v
-    -> ReadWord stn (Mem st) a = v.
+    -> ReadWord stn (Mem st) a = Some v.
   rewrite sepFormula_eq; intros.
   apply H0 in H; clear H0; propxFo.
-  unfold ReadWord. simpl in *.
+  unfold ReadWord, mem_get_word, footprint_w, ReadByte. simpl in *.
   repeat match goal with
            | [ H : _ |- _ ] => apply smem_get_read in H; rewrite H
          end.
-  auto.
+  congruence.
 Qed.
 
 
