examples/Baby.v
@@ -81,7 +81,7 @@ Section final.
   Definition final := Eval compute in exec immedSettings immedProgram 20
     (proj1_sig immedProgReallyOk,
       {| Regs := fun _ => wzero _;
-        Mem := fun _ => wzero _ |}).
+        Mem := fun _ => Some (wzero _) |}).
 
   Eval compute in match final with None => wzero _ | Some (_, final') => Regs final' Rp end.
 End final.
